compiler/proofs/compilerProofScript.sml
@@ -12,9 +12,8 @@ val config_ok_def = Define`
   config_ok (cc:α compiler$config) mc ⇔
     env_rel prim_tenv cc.inferencer_config.inf_env ∧
     prim_tdecs = convert_decls cc.inferencer_config.inf_decls ∧
-    cc.backend_config.source_conf = ((prim_config cc.backend_config.clos_conf.max_app):α backend$config).source_conf ∧
-    cc.backend_config.mod_conf = ((prim_config cc.backend_config.clos_conf.max_app):α backend$config).mod_conf ∧
-    cc.backend_config.clos_conf = ((prim_config cc.backend_config.clos_conf.max_app):α backend$config).clos_conf ∧
+    cc.backend_config.source_conf = (prim_config:α backend$config).source_conf ∧
+    cc.backend_config.mod_conf = (prim_config:α backend$config).mod_conf ∧
     0 < cc.backend_config.clos_conf.max_app ∧
     backendProof$conf_ok cc.backend_config mc`;
 
@@ -24,9 +23,8 @@ val initial_condition_def = Define`
     type_sound_invariants (NONE:(unit,v) semanticPrimitives$result option) (st.tdecs,st.tenv,st.sem_st,st.sem_env) ∧
     env_rel st.tenv cc.inferencer_config.inf_env ∧
     st.tdecs = convert_decls cc.inferencer_config.inf_decls ∧
-    cc.backend_config.source_conf = ((prim_config cc.backend_config.clos_conf.max_app):α backend$config).source_conf ∧
-    cc.backend_config.mod_conf = ((prim_config cc.backend_config.clos_conf.max_app):α backend$config).mod_conf ∧
-    cc.backend_config.clos_conf = ((prim_config cc.backend_config.clos_conf.max_app):α backend$config).clos_conf ∧
+    cc.backend_config.source_conf = (prim_config:α backend$config).source_conf ∧
+    cc.backend_config.mod_conf = (prim_config:α backend$config).mod_conf ∧
     0 < cc.backend_config.clos_conf.max_app ∧
     backendProof$conf_ok cc.backend_config mc`;
 
@@ -151,19 +149,12 @@ val compile_correct_gen = Q.store_thm("compile_correct_gen",
       |> GEN_ALL
       |> drule)
   \\ simp[]
-  \\ simp[GSYM AND_IMP_INTRO]
-  \\ simp[RIGHT_FORALL_IMP_THM]
-  \\ impl_tac >- metis_tac[]
-  \\ impl_tac >- metis_tac[]
-  \\ simp[GSYM RIGHT_FORALL_IMP_THM,AND_IMP_INTRO,GSYM CONJ_ASSOC]
-  \\ ONCE_REWRITE_TAC[CONJ_COMM]
-  \\ simp[GSYM AND_IMP_INTRO] (* TODO: why is this necessary? *)
   \\ disch_then drule
   \\ disch_then(qspec_then`st.sem_st.ffi`mp_tac o CONV_RULE (RESORT_FORALL_CONV (sort_vars["ffi"])))
   \\ qpat_assum`_ = THE _`(assume_tac o SYM)
   \\ simp[]
   \\ disch_then (match_mp_tac o MP_CANON)
-  \\ conj_tac >- fs []
+  \\ simp[RIGHT_EXISTS_AND_THM]
   \\ fs[can_type_prog_def]
   \\ Cases_on`prog_diverges st.sem_env st.sem_st (prelude ++ x)`
   >- metis_tac[semanticsPropsTheory.prog_diverges_semantics_prog]
